---
layout: post
title: "Differential Geometry, Part 6"
author: "Jay Havaldar"
date:   2017-07-18
mathjax: true
category: [math]
download: true
category: notes
---

# Part VI: Geometry of Surfaces in $\mathbb{R}^3$

We continue by analogy. First, we set up the essential machinery for discussing curves in $\mathbb{R}^3$, such as frame fields, connection forms, and the structural equations in Part II. Then in Part III, we discussed the geometry of $\mathbb{R}^3$, or more specifically, the unique properties which are preserved by Euclidean isometries. Similarly, in Part V we discussed the machinery for discussing surfaces in $\mathbb{R}^3$, namely the shape operator. And in Part VI we will discuss the intrinsic geometry of a surface in $\mathbb{R}^3$, concluding as we did Part III with a congruence theorem for surfaces. Man, it's like poetry. Makes me tear up.

## The Fundamental Equations

Once more, the Cartan equations from Part II find their use. As with the Frenet frame approach, we first need to set up a system of frames on $M$.

**Definition:** An **adapted frame field** $E_i$ on a region $\mathcal{O}$ in $M \subset \mathbb{R}^3$ is a Euclidean frame field (three orthonormal vector fields) such that $E_3$ is always normal to $M$.

##### Lemma

On a region $\mathcal{O}$ in $M \subset \mathbb{R}^3$, there exists an adapted frame field if and only if $\mathcal{O}$ is orientable and there exists a non-vanishing tangent vector field on $\mathcal{O}$.

This condition is clearly necessary, since the orientable condition guarantees the existence of a unit normal vector field (see: Part IV), and the tangent space condition guarantees us the remaining two vector fields. From a unit vector field $U$ and a tangent vector $V$, we can define a frame:

<p>
$$\begin{aligned}
E_1 &= \frac{V}{\vert V \vert} \\
E_2 &= U \times E_1 \\
E_3 &= U
\end{aligned}$$
</p>

This lemma immediately implies that on the image of any patch in $M$, there is an adapted frame field on $M$ in an open region. Thus adaptable frame fields exist on surfaces, at least locally.

Suppose $E_i$ are an adapted frame field on $M$. We can extend the frame field so that it is defined on an open set in $\mathbb{R}^3$. Now, we look at the connection equations: 

<p>
$$\begin{aligned}
\nabla_v E_i = \sum \omega_{ij}(v) E_j
\end{aligned}$$
</p>

This definition really only makes sense if we apply them to tangent vectors $v$ to $M$. Now, we have a set of $1$-forms defined on $M$.

Again, $\omega_{ij}(v)$ defines the initial rate at which $E_i$ rotates towards $E_j$ as $p$ moves in the direction $v$.

##### Corollary

As a corollary, we can define the shape operator in terms of the connection forms, since $E_3 = U$ is a unit normal vector field. Then:

<p>
$$\begin{aligned}
S_p(v) = \omega_{13}(v)E_1(p) + \omega_{23}E_2(p)
\end{aligned}$$
</p>

This follows directly from the connection equations.

We also can carry over directly the **dual** $1$ **-forms**, $\theta_i(v) = v\cdot E_i$, as long as we restrict $v$ to tangent vectors to $M$. This means that in particular, $\theta_3(v) = 0$, since $E_3$ does not lie in the tangent plane. Thus, due to skew-symmetry, we essentially only have five $1$-forms:

- $\theta_1, \theta_2$ are dual to the tangent vector fields $E_1, E_2$.
- $\omega_{12}$ gives the rate of rotation of $E_1$ towards $E_2$.
- $\omega_{13}, \omega_{23}$ completely describe the shape operator.

##### Theorem

The big one! If $E_i$ is an adapted frame field on $M \subset \mathbb{R}^3$, then its dual forms and connection forms satisfy:

**First Structural Equations**

<p>
$$\begin{aligned}
d \theta_1 &= \omega_{12} \wedge \theta_2 \\
d \theta_2 &= \omega_{21} \wedge \theta_1
\end{aligned}$$
</p>

**Gauss Equation**

<p>
$$\begin{aligned}
d \omega_{12} = \omega_{13} \wedge \omega_{32}
\end{aligned}$$
</p>

**Codazzi Equations**

<p>
$$\begin{aligned}
d \omega_{13} = \omega_{13} \wedge \omega_{23} \\
d \omega_{23} = \omega_{21} \wedge \omega_{13}
\end{aligned}$$
</p>

The first structural equations are the same as in Part II. The second structural equations imply the Gauss equations and the Codazzi equations, the former of which describes the rotation between $E_1, E_2$ and the latter of which describes the shape operator. It is important to note that these equations depend on the choice of frame field.

Since the corresponding connection forms describe the shape operator, the Codazzi equations describe the rate at which the shape of $M$ is changing.

##### Lemma

We can describe geodesics using connection forms. Let $\alpha$ be a unit speed curve in $M$. If $E_1, E_2, E_3$ is an adapted frame field where $E_1 = T$ along $\alpha$ ($T$ being the unit tangent vector from the Frenet frame), we claim that $\alpha$ is a geodesic if and only if $\omega_{12}(T) = 0$.

First, denote $E_i' = E_i(\alpha(t))$ at $t=0$. But this is the same as the covariant derivative: $E_i' = \nabla_{\alpha'} E_i$. In particular for this curve, $\alpha' = T$.

Since $E_i$ is an adapted frame field and $T$ is a unit vector, $E_i'$ must be entirely in the diretction of $E_2$. This means that: $\omega_{12}(T) = (\nabla_T E_1) \cdot E_2$. But since $\alpha$ is a geodesic, $\alpha''$ is normal to $M$; so there is no such component in the $E_2$ direction, so indeed $\omega_{12}(T) = 0$.

So, the connection forms already find some use in making sense of curves on surfaces.

## Form Computations

If $E_1, E_2, E_3$ is an adapted frame field on $M \subset \mathbb{R}^3$, we say that $E_1, E_2$ constitute a tangent frame field on $M$. So any tangent vector field $V$ on $M$ can be decomposed into its components $V \cdot E_1, V\cdot E_2$ along each of the tangent frames.

Thus, to show that two forms are equal, we just have to compare them on basis vector fields $E_1, E_2$. So now we can equivalently form a "basis" of forms on $M$.

##### Lemma

Let $\theta_1, \theta_2$ be the dual $1$-forms of $E_1, E_2$ on $M$. If $\phi$ is a $1$-form and $\psi$ a $2$-form, then:

<p>
$$
\phi = \phi(E_1) \theta_1 + \phi(E_2) \theta_2
$$
</p>
<p>
$$
\mu = \mu(E_1, E_2) \theta_1 \wedge \theta_2
$$
</p>

The first statement comes easily from the criteria for equality of frame fields; the second comes from our definition of the wedge product:

<p>
$$\begin{aligned}
\theta_1 \wedge \theta_2(E_1, E_2) &= \theta_1(E_1) \theta_2(E_2) - \theta_1 (E_2) \theta_2 (E_1) \\
&= 1
\end{aligned}$$
</p>

##### Lemma

<p>
$$
\omega_{13} \wedge \omega_{23} = K \theta_1 \wedge \theta_2
$$
</p>
<p>
$$
\omega_{13} \wedge \theta_2 + \theta_1 \wedge \omega_{23} = 2H \theta_1 \wedge \theta_2
$$
</p>

To prove these equations, first we need to write a matrix representation of the shape operator $S$. From the connection equations:

<p>
$$\begin{aligned}
S(E_1) &= -\nabla_{E_1} E_3 = \omega_{13}(E_1) E_1 + \omega_{23}(E_1) E_2 \\
S(E_2) &= -\nabla_{E_2} E_3 = \omega_{13}(E_1) E_1 + \omega_{23}(E_1) E_2 
\end{aligned}$$
</p>

So the matrix of $S$ is then:

<p>
$$
\begin{bmatrix}
\omega_{13} (E_1) & \omega_{13} (E_2)\\
\omega_{23} (E_1) & \omega_{23} (E_2)
\end{bmatrix}$$
</p>

Now, we test equality of forms in the usual way. For the first form:

<p>
$$\begin{aligned}
(\omega_{13} \wedge \omega_{23})(E_1, E_2) &= \omega_{13}(E_1)\omega_{23}(E_2) - \omega_{13}(E_2) \omega_{23}(E_1) \\
&= \det S \\
&= K
\end{aligned}$$
</p>

And similarly for the second form:

<p>
$$\begin{aligned}
(\omega_{13}\wedge \theta_2 + \theta_1\wedge \omega_{23})(E_1, E_2) &= \omega_{13}(E_1) + \omega_{23}(E_2) \\
&= \text{tr} S \\
&= 2H
\end{aligned}$$
</p>

And from the first half of this lemma and the Gauss equation, we get:

<p>
$$\begin{aligned}
d \omega_{12} = -K \theta_1 \wedge \theta_2
\end{aligned}$$
</p>

Which we will call the second structural equation. Since $\omega_{12}$ is something like the rate of rotation of the tangent frame field $E_1, E_2$, its derivative $K$ measures something like a second derivative of $E_1, E_2$.

**Definition:** A **principal frame field** on $M$ is an adapted frame field so that $E_1, E_2$ are principal vectors of $M$.

Where there are no umbilic points, there is a unique principal frame on $M$ up to changes in sign. We leave this proof out, but it's not hard to prove using linear algebra and some analysis.

Suppose we have a principal frame field on $M$, then we can rename the principal directions so that $S(E_1) = k_1 E_1$ and $S(E_2) = k_2 E_2$. Thus by the basis formula from earlier, we have:

<p>
$$\begin{aligned}
\omega_{13} &= k_1 \theta_1 \\
\omega_{23} &= k_2 \theta_2
\end{aligned}$$
</p>

This leads us to an interesting corollary of the Codazzi equations.

##### Theorem

If $E_1, E_2, E_3$ is a principal frame field on $M$, then:

<p>
$$\begin{aligned}
E_1[k_2] = (k_1 - k_2) \omega_{12}(E_2) \\
E_2[k_1] = (k_1 - k_2) \omega_{12}(E_1)
\end{aligned}$$
</p>

We can prove this just with differential forms algebra. First, we apply the Codazzi equations:

<p>
$$\begin{aligned}
d(\omega_{13}) = d(k_1 \theta_1) & =\omega_{12} \wedge \omega_{23}  \\
dk_1 \wedge \theta_1 + k_1 d\theta_1 &= k_2 \omega_{12} \wedge \theta_2 \\
\end{aligned}$$
</p>

But we also know from the First Structural Equations that $d \theta_1 = \omega_{12} \wedge \theta_2$. So finally we have:

<p>
$$\begin{aligned}
dk_1 \wedge \theta_2 = (k_2 - k_1) \omega_{12} \wedge \theta_2
\end{aligned}$$
</p>

To prove this statement, we simply apply each of the $2$-forms to $(E_1, E_2)$:

<p>
$$\begin{aligned}
(dk_1 \wedge \theta_2)(E_1, E_2) &= (k_2 - k_1) \omega_{12} \wedge \theta_2 (E_1, E_2) \\
-dk_1(E_2) &= (k_2 - k_1) \omega_{12} (E_1)
\end{aligned}$$
</p>

Therefore:

<p>
$$\begin{aligned}
E_2[k_1] = dk_1(E_2) = (k_1 - k_2) \omega_{12} (E_1)
\end{aligned}$$
</p>

And similarly for the second statement.

## Some Global Theorems

We know apply our knowledge of the shape operator to draw some conclusions of (connected) surfaces.

##### Theorem

If $S$ is identically zero, then $M$ is part of the plane in $\mathbb{R}^3$.

This means that the unit vector field $E_3$ is the same vector everywhere. So, we pick a fixed point $p$ in $M$ and consider any other point $q$ in $M$, and draw a curve $\alpha$ in $M$ so that $\alpha(0) = p, \alpha(1) = q$. So we consider the function:
<p>
$$\begin{aligned}
f(t) &= (\alpha(t) - p)\cdot E_3 \\
\frac{df}{dt} &= \alpha' \cdot E_3 = 0
\end{aligned}$$
</p>

So indeed, since $f(0) = 0$, $f$ is identically zero. By checking $f(1)$, we see that indeed $(q-p)\cdot E_3 = 0$, so that indeed, $q$ lies in the plane normal to $E_3$.

##### Theorem

If $M$ is umbilic everywhere, then $M$ has constant Gaussian curvature.

To prove this, for each region in $M$ we pick an adapted frame field $E_1, E_2, E_3$. Since every direction is a principal direction, indeed this is a principal frame field. So our earlier lemma from the Codazzi equations in the previous section, we have:
<p>
$$\begin{aligned}
dk(E_1) = dk(E_2) = 0
\end{aligned}$$
</p>

By the basis formulas, $dk = 0$ in the region. But then we know that $dK = d(k_1^2) = 2k_1 dk$ = 0. So indeed, we have shown that $K$ is constant everywhere since $dK=0$ in every region of $M$.

##### Theorem

If $M$ is umbilic everywhere, and $K > 0$, then $M$ is part of a sphere in $\mathbb{R}^3$ of radius $\frac{1}{\sqrt{K}}$.

To prove this theorem, We will construct a point which is equidistant from every point in $M$. Pick any point $p$ of $M$ and denote the unit normal $E_3$. Then we claim that the center is:

<p>
$$\begin{aligned}
c = p + \frac{1}{k(p)} E_3(p)
\end{aligned}$$
</p>

Now, we pick any point $q$ of $M$, and draw a curve $\alpha$ in $M$ as in the preceding proof with $\alpha(0) = p, \alpha(1) =q$. We extend $E_3$ to a unit normal vector field all along $\alpha$. Now all we have to do is consider the curve:

<p>
$$\begin{aligned}
\gamma = \alpha + \frac{1}{k} E_3
\end{aligned}$$
</p>

How do we know $k$ is a constant? Well, since $E_3$ was extended continuously, $k(p)$ is also continuous; but our previous theorem tells us that the Gaussian curvature $K=k^2$ is constant. Taking the derivative of $\gamma$, we get:

<p>
$$\begin{aligned}
\gamma' = \alpha' + \frac{1}{k} E_3'
\end{aligned}$$
</p>

But by the definition of the shape operator (which we recall is just scalar multiplication at umbilic points):

<p>
$$\begin{aligned}
E_3' = -S(\alpha') = -k\alpha'
\end{aligned}$$
</p>

So indeed $\gamma' = 0$, and $\gamma$ is constant. So in particular: 

<p>
$$\begin{aligned}
\gamma(0) = p +\frac{1}{k}E_3 = \gamma(1) = q+\frac{1}{k}E_3
\end{aligned}$$
</p>

And in particular, $\vert c-p \vert = \vert c - q \vert$. Furthermore, since $K = k^2$, the distance is indeed $\frac{1}{\sqrt{K}}$.

Combining the three previous theorems: A surface is all-umbilic if and only if $M$ is a part of a plane or sphere.

##### Corollary

A compact all-umbilic surface is a sphere.

First, we note from topology that a connected surface has only two clopen sets: i


---
